\input doc/format
\notespagesize

\def\loss{{\rm Loss}}
\def\dv{{\rm d}}

% {{{1 Section Problem
\section{Problem}

Given predictions ${\bf p} = [p_1, p_2, \ldots, p_n]$ and targets
${\bf y} = [y_1, y_2, \ldots, y_n]$, the cross entropy loss is defined as
%
$$
    \loss = - \sum_{i} y_i \log p_i,
$$
with gradient:
%
$$
    {\dv \loss \over \dv p_i} = - {\dv y_i \log p_i \over \dv p_i} = - {y_i \over p_i }.
$$

However, this gradient is not numerical stable, as for any super small $p_i$,
i.e., $p_i \to 0$, the gradient is \symbol{NaN}.

\section{Solution}

A common trick to solve this is calculating the gradient from loss $\loss$
w.r.t.~the logits $o_i$  directly, where
%
$$
    p_i = {\exp^{o_i} \over \sum_k \exp^{o_k}}.
$$

The gradient, w.r.t.~logits, is
%
$$
    {\dv \loss \over \dv o_i} =
         - \sum_k {\dv \loss \over \dv p_k} {\dv p_k \over \dv o_i}.
$$
where
%
$$
    {\dv \loss \over \dv p_k} = - {y_k \over p_k},
$$
and
%
$$
    {\dv p_k \over \dv o_i} =
        \cases { p_i (1-p_i), & if $k=i$; \cr
                 -p_k p_i & if $k\neq i$. \cr }
$$

Substituting everything into the loss gradient, we get
%
$$
    \eqalign{{\dv \loss \over \dv o_i}
        & = (\dots) \cr
        & = \left( p_i \sum_k { y_k} \right) - y_i \cr
        & = p_i - y_i \cr
    }
$$
where $\sum_k { y_k} = 1$ given ${\bf y}$ is target probability.

\section{Numerical Stable}

Now let's revisit the loss function with respect to the logits.
%
$$
    \eqalign{
      \loss & = - \sum_{i} y_i \log p_i, \cr
            & = - \sum_{i} \left(
                y_i \log {\exp^{o_i} \over \sum_k \exp^{o_k}}
              \right)\cr
    }
$$
For any large logit $o_k$, the $\exp$ is $\inf$, so unstable. The common trick
is to find the max item $o_{max}=\max_k o_k$, and subtract it from all $o_k$s,
i.e.,
$$
    \eqalign{
      \loss & = - \sum_{i} \left(
                y_i \log {\exp^{o_i} \over \sum_k \exp^{o_k}}
                \right)\cr
            & = - \sum_{i} \left(
                y_i \log {\exp^{o_i-o_{max}} \over \sum_k \exp^{o_k-o_{max}}}
                \right)\cr
            & = -
                \left(
                   \sum_{i} y_i (o_i-o_{max})
                \right)
                + \log\left(
                    \sum_k \exp^{o_k-o_{max}}
                 \right)
              \cr
    }
$$

\vfill
\bye
